\documentclass[10pt,a4paper]{article}
\usepackage[utf8]{inputenc}
\usepackage[english]{babel}
\usepackage{amsmath}
\usepackage{amsfonts}
\usepackage{amssymb}
\usepackage{graphicx}
\begin{document}
\subsection*{Exercise 1}
\paragraph{a)}
\begin{align*}
E_{kin} &= \gamma m_0 c^2 - m_0 c^2 = m_0 c^2 (\gamma - 1) \\
\frac{E_{kin}}{m_0 c^2} &= \frac{1}{\sqrt{1-\beta^2}} - 1 \\
\beta &= \sqrt{1-\left(\frac{E_{kin}}{m_0 c^2} + 1\right)^{-2}}
\end{align*}
Now rewriting the energy density as
\begin{align*}
\rho_E = \rho_{E_0} + \rho_{E_{kin}}
\end{align*}
where $\rho_{E_0}$ is the energy density occurring from the rest mass and $\rho_{E_{kin}}$ is the kinetic energy density. Analogous to the calculation in the script one gets:
\begin{align*}
\rho_E &= \rho_{E_0} + \int_{E_{min}}^\infty dE_{kin}\ \frac{dn_{CR}}{dE_{kin}}E_{kin}\\
&=\rho_{E_0} + \int_{E_{min}}^\infty dE_{kin}\ \frac{4\pi}{\beta c}\frac{d\Phi}{dE_{kin}}E_{kin}\\
&=\rho_{E_0} + \frac{4\pi \Phi_0}{c} \int_{E_{min}}^\infty dE_{kin}\ \frac{E_{kin}^{-\gamma+1}}{\sqrt{1-\left(\frac{E_{kin}}{m_0 c^2} + 1\right)^{-2}}}\\
\end{align*}
In the last step the power-law for the kinetic energy flux is inserted and the expression for $\beta$ from before.

\paragraph{b)}
From the graph one can read the points $P_1 = (10 | 2\cdot 10^{-3})$ and $P_2=(10^2 | 5 \cdot 10^{-6})$. This results in $\Phi_0 = 0.8\ (cm^2\ s\ sr\ GeV)^{-1}$ and $\gamma = 2.602$.

\paragraph{c)}
Inserting into the integral in b) gives a value
\begin{align*}
\int_{E_{min}}^\infty dE_{kin}\ \frac{E_{kin}^{-\gamma+1}}{\sqrt{1-\left(\frac{E_{kin}}{m_0 c^2} + 1\right)^{-2}}} = 1.7323
\end{align*}
Resulting in $\rho_E = $
\end{document}